forloop.v
@@ -1,0 +1,96 @@
+From iris.program_logic Require Import weakestpre.
+From iris.heap_lang Require Import proofmode notation.
+From iris.proofmode Require Import tactics.
+
+(** This definition is quite tricked in order to make the bind rule work. When
+having:
+
+  for: i := e1 to e2 do e3
+
+We want to be able to use the bind rule in [e1] and [e2]. In order to do so,
+we cannot make [forloop] in [e1] and [e2], but we instead let it take a tuple
+consisting of [e1] and [e2]. *)
+Definition forloop : val :=
+  (rec: "go" "ij" "f" :=
+    if: Fst "ij" < Snd "ij"
+    then "f" (Fst "ij");; "go" (#1 + Fst "ij", Snd "ij") "f"
+    else #()).
+
+Notation "'for:' i := e1 'to' e2 'do' e3" :=
+  (forloop (e1,e2) (λ: i, e3))%E
+  (at level 200, i at level 1, e1, e2, e3 at level 200) : expr_scope.
+
+(* Since tactics like [simpl_subst] and [solve_closed] cannot deal with open
+terms (i.e. terms in which binders are Coq variables instead of actual strings),
+we parametrize this lemma by a value [v] (all values are closed, and
+[simpl_subst] and [solve_closed] know about that) and an equality [v = λ: i, e].
+Only when we actually want to use the lambda rule, we rewrite using the 
+equality. *)
+Lemma wp_forloop_true `{heapG Σ} E v i e (n m : Z) Φ `{Closed [i] e} :
+  n < m →
+  v = (λ: i, e)%V →
+  ▷ WP subst i #n e @ E {{ _, WP forloop (#(1 + n), #m) v @ E {{ Φ }} }}-∗
+  WP forloop (#n,#m) v @ E {{ Φ }}.
+Proof.
+  iIntros (? Hv) "Hwp". wp_rec. wp_let. do 2 wp_proj. wp_op=> ?; [|lia]. wp_if.
+  wp_proj. rewrite {3}Hv. wp_lam. iApply (wp_wand with "Hwp").
+  iIntros (w) "Hwp". wp_seq. wp_proj. wp_op. wp_proj. done.
+Qed.
+
+Lemma wp_forloop_false `{heapG Σ} E (v : val) (n m : Z) Φ :
+  m ≤ n →
+  ▷ Φ #() -∗ WP forloop (#n,#m) v @ E {{ Φ }}.
+Proof.
+  iIntros (?) "HΦ". wp_rec. wp_let. do 2 wp_proj. wp_op=> ?; [lia|]. by wp_if.
+Qed.
+
+Lemma wp_for_true `{heapG Σ} E i (n m : Z) e Φ `{Closed [i] e} :
+  n < m →
+  ▷ WP subst i #n e @ E {{ _, WP for: i := #(1 + n) to #m do e @ E {{ Φ }} }}-∗
+  WP for: i := #n to #m do e @ E {{ Φ }}.
+Proof. intros. eapply (wp_forloop_true E (LamV i e) i e); by unlock. Qed.
+
+Lemma wp_for_false `{heapG Σ} E i (n m : Z) e Φ `{Closed [i] e} :
+  m ≤ n →
+  ▷ Φ #() -∗ WP for: i := #n to #m do e @ E {{ Φ }}.
+Proof. intros. by apply (wp_forloop_false E (LamV i e)). Qed.
+
+Lemma wp_for `{heapG Σ} E m n e en j P `{Closed [j] e} `{Closed [] en}:
+  (m ≤ n)%Z ->
+  WP en @ E {{v, ⌜v = #n⌝}} -∗ P m -∗
+     □(∀ (i : Z), ⌜m ≤ i < n⌝%Z -∗ P i -∗ ▷ WP (subst' j #i e) @ E {{_, P (1 + i)%Z}}) -∗
+     WP for: j := #m to en do e @ E {{_, P n}}.
+Proof.
+  intros HLeq.
+  iIntros "Hend H H'" ; iCombine "H" "H'" as "H".
+  iDestruct (wp_frame_l _ en _ _ with "[H Hend]") as "H" ;  first (iSplitL "H" ; [iExact "H" | iExact "Hend"]).
+  wp_bind en ; iApply wp_mono; last iExact "H".
+  iIntros (v) "[[HPm HInv] %]" ; subst ; simpl.
+  iRevert (HLeq). 
+  iRevert "HPm".
+  iRevert "HInv".
+  iRevert (m).
+  iLöb as "HLöb".
+
+  iIntros (m) "#HInv HPm %".
+  destruct (decide (m = n)) ; subst.
+  - iApply wp_for_false ; done.
+  - iApply wp_for_true ; first lia.
+    iAssert (⌜m ≤ m ∧ m < n⌝)%I as "HBoth". 
+    { iPureIntro ; split; [reflexivity | lia]. }
+    iDestruct ("HInv" $! m with "HBoth HPm") as "H".
+    iNext.
+    iAssert (□∀ i : Z, ⌜m ≤ i ∧ i < n⌝ -∗ P i -∗ ▷ WP subst j #i e @ E {{ _, P (1 + i) }})%I as "HInvBoxed" ; first done.
+    iCombine "HLöb" "HInvBoxed" as "HH".
+    iDestruct (wp_frame_l _ _ _ _ with "[HH H]") as "H" ; first  (iSplitL "HH" ; [iExact "HH" | iExact "H"]).
+    iApply wp_mono ; last iExact "H".
+    simpl.
+    iIntros (v) "[[HInv HLöb] HPm]".
+    iDestruct ("HInv" $! (1 + m)) as "HHH".
+    destruct (decide (1 + m = n)) ; subst.
+    + iApply wp_for_false ; (done || lia).
+    + iDestruct ("HHH" with "[HLöb ]") as "HTemp".
+      iDestruct "HLöb" as "#HLöb" ; iAlways.
+      iIntros (i) "%" ; iApply "HLöb" ; iPureIntro ; lia.
+      iApply ("HTemp" with "HPm") ; iPureIntro ; lia.
+Qed.    
