iterators/util.v
@@ -1,0 +1,116 @@
+From mathcomp Require Import ssreflect.
+From iris.prelude Require Import fin_collections listset_nodup.
+
+Definition collection_sum_with `{Elements A C} (f : A -> nat) : C -> nat :=
+      collection_fold (fun a n => n + f a) 0.
+ 
+ Instance collection_sum_with_proper `{FinCollection A C} (f : A -> nat) : Proper ((≡) ==> (=)) (collection_sum_with f : C -> nat).
+ Proof.
+   unfold collection_sum_with.
+   apply (collection_fold_proper).
+   apply eq_equivalence.
+   solve_proper.
+   intros. lia.
+ Qed.
+ 
+ Lemma collection_sum_with_empty `{FinCollection A C} f :
+   collection_sum_with f ∅ = 0.
+ Proof.
+      unfold collection_sum_with, collection_fold. simpl.
+      rewrite elements_empty. done.
+ Qed.
+ 
+ Lemma collection_sum_with_singleton_union `{FinCollection A C} x D f :
+   x ∉ D ->
+   collection_sum_with f ({[x]} ∪ D) = f x + collection_sum_with f D.
+ Proof.
+   intro. 
+   unfold collection_sum_with, collection_fold. simpl.
+   rewrite (foldr_permutation (=) (λ (a : A) (n : nat), n + f a) 0 _ (elements ({[x]} ∪ D))(x :: elements D)) ; [|intros ; lia|].
+   simpl. lia.
+   by apply elements_union_singleton.  
+ Qed.
+ 
+ Lemma collection_sum_with_subseteq_le `{FinCollection A C} `{forall x D, Decision (x ∈ D)} (D1 D2 : C) f :
+   D1 ⊆ D2 ->
+   collection_sum_with f D1 ≤ collection_sum_with f D2. 
+ Proof.
+   apply (collection_ind
+            (fun D1 => forall D2,
+                 D1 ⊆ D2 ->
+                 collection_sum_with f D1 ≤ collection_sum_with f D2)). 
+   { intros ? ? Heq. apply forall_proper. intros.
+     rewrite subseteq_proper ; [|done..].
+     by rewrite (collection_sum_with_proper f _ _ Heq ).
+   }
+   - clear D1 D2.
+     intros D2 _. rewrite collection_sum_with_empty. lia.
+   - clear D1 D2.
+     intros x D1 Hx IH D2 Hsubset.
+     rewrite (union_difference {[x]} D2) ; [|set_solver].
+     rewrite collection_sum_with_singleton_union.
+     rewrite collection_sum_with_singleton_union.
+     assert (D1 ⊆ D2 ∖ {[x]}) as Hsubset'. set_solver.
+     specialize (IH (D2 ∖ {[x]}) Hsubset').
+     lia. set_solver. assumption.
+ Qed.
+ Lemma collection_sum_with_union `{FinCollection A C} `{forall x D, Decision (x ∈ D)} D1 D2 f :
+   collection_sum_with f (D1 ∪ D2) =
+   (collection_sum_with f D1 + collection_sum_with f D2) - collection_sum_with f (D1 ∩ D2).
+ Proof.
+   apply (collection_ind (fun D => collection_sum_with f (D ∪ D2) =
+                                   (collection_sum_with f D + collection_sum_with f D2) - collection_sum_with f (D ∩ D2))).
+   {
+     intros X Y ?. rewrite union_proper ; [|done..].
+     rewrite intersection_proper ; [|done..].
+       by rewrite (collection_sum_with_proper _ X Y).
+   }
+   - rewrite intersection_empty_l union_empty_l collection_sum_with_empty .
+     lia.
+   - intros x D HnIn IH.
+     rewrite collection_sum_with_singleton_union ; [|assumption].
+     
+     destruct (decide (x ∈ D2)) as [HD2|HD2].
+     + rewrite {1}[{[x]} ∪ D]union_comm -union_assoc (subseteq_union_1 {[x]} D2).
+       rewrite intersection_union_r. rewrite (subseteq_intersection_1 {[x]} D2).
+       rewrite collection_sum_with_singleton_union.
+       rewrite IH. lia.
+       rewrite not_elem_of_intersection. by left.
+       apply elem_of_subseteq_singleton. assumption.
+       apply elem_of_subseteq_singleton. assumption.
+     + rewrite -union_assoc.
+       rewrite collection_sum_with_singleton_union.
+       rewrite intersection_union_r. rewrite (_:{[x]} ∩ D2 ≡ ∅).
+       rewrite union_empty_l. rewrite IH.
+       pose proof (collection_sum_with_subseteq_le (D ∩ D2) D f (intersection_subseteq_l _ _)).
+       lia. set_solver. set_solver.
+ Qed.
+ 
+ Lemma collection_sum_with_domains `{FinCollection A C} D f g :
+   (forall x, x ∈ D -> f x = g x) ->
+   collection_sum_with f D = collection_sum_with g D.
+ Proof.
+   apply (collection_ind (fun D => (forall x, x ∈ D -> f x = g x) ->
+                                   collection_sum_with f D = collection_sum_with g D)).
+   { intros ? ? Heq.
+     rewrite (collection_sum_with_proper f _ _ Heq).
+     rewrite (collection_sum_with_proper g _ _ Heq).
+     split. intros Hother Hdom. apply Hother. intro. rewrite elem_of_proper ;[|done..]. apply Hdom.
+     intros Hother Hdom. apply Hother. intro. rewrite elem_of_proper ;[|done..]. apply Hdom.
+   }
+   - intro. rewrite collection_sum_with_empty.
+     symmetry. apply collection_sum_with_empty.
+   - clear D. intros x D Hx IH Hdom. 
+     rewrite collection_sum_with_singleton_union ; [|assumption].
+     rewrite collection_sum_with_singleton_union ; [|assumption].
+     rewrite Hdom ; [|set_solver].
+     rewrite IH. done.
+     intros ? ?. apply Hdom. set_solver.
+ Qed.        
+
+ Instance listset_nodup_dec_elem_of `{EqDecision A} x (C : listset_nodup A) : Decision (x ∈ C) :=
+   elem_of_list_dec x (elements C).
+ 
+
+    
+    
